Add Intermediary to prove Complete.

C1_Schreier_vector.v
@@ -10,14 +10,14 @@ Definition vector := fmap perm.
 (* Add all numbers reachable from i. *)
 Fixpoint extend (i : positive) (h : perm)
   (gen : list perm) (V : vector)
-  (dst : list positive) :=
+  (new : list positive) :=
   match gen with
-  | [] => (V, dst)
+  | [] => (V, new)
   | g :: gen' =>
     let j := g⋅i in
     match lookup V j with
-    | Some _ => extend i h gen' V dst
-    | None => extend i h gen' (insert V j (g ∘ h)) (j :: dst)
+    | Some _ => extend i h gen' V new
+    | None => extend i h gen' (insert V j (g ∘ h)) (j :: new)
     end
   end.
 
@@ -25,27 +25,27 @@ Fixpoint extend (i : positive) (h : perm)
 Variable gen : list perm.
 
 (* Extend all numbers in the source list. *)
-Fixpoint extend_loop (V : vector) (src dst : list positive) :=
-  match src with
-  | [] => (V, dst)
-  | i :: src' =>
+Fixpoint extend_loop (V : vector) (try new : list positive) :=
+  match try with
+  | [] => (V, new)
+  | i :: try' =>
     match lookup V i with
-    | None => extend_loop V src' dst
+    | None => extend_loop V try' new
     | Some h =>
-      match extend i h gen V dst with
-      | (V', dst') => extend_loop V' src' dst'
+      match extend i h gen V new with
+      | (V', new') => extend_loop V' try' new'
       end
     end
   end.
 
 (* Repeat orbit extension n times. *)
-Fixpoint loop (V : vector) (src : list positive) (n : nat) :=
+Fixpoint loop (V : vector) (try : list positive) (n : nat) :=
   match n with
   | O => V
   | S m =>
-    match extend_loop V src [] with
+    match extend_loop V try [] with
     | (V', []) => V'
-    | (V', src') => loop V' src' m
+    | (V', new) => loop V' new m
     end
   end.
 
@@ -78,11 +78,11 @@ Definition Sound (V : vector) := ∀i,
   | None => True
   end.
 
-Lemma sound_extend h gen' V dst :
+Lemma sound_extend h gen' V new :
   Generates gen h -> gen' ⊆ gen ->
-  Sound V -> Sound (fst (extend h⋅k h gen' V dst)).
+  Sound V -> Sound (fst (extend h⋅k h gen' V new)).
 Proof.
-revert V dst; simple_ind gen'.
+revert V new; simple_ind gen'.
 apply incl_cons_inv in H0 as [].
 destruct (lookup _); apply IHgen'; try easy.
 intros j; rewrite lookup_insert.
@@ -90,23 +90,23 @@ destruct (_ =? _) eqn:E; [convert_bool; subst; split|apply H1].
 apply compose_generator; easy. apply apply_compose.
 Qed.
 
-Lemma sound_extend_loop V src dst :
-  Sound V -> Sound (fst (extend_loop V src dst)).
+Lemma sound_extend_loop V try new :
+  Sound V -> Sound (fst (extend_loop V try new)).
 Proof.
-revert V dst; simple_ind src.
-destruct (lookup V a) eqn:E. destruct (extend _) as [V' dst'] eqn:E'.
-replace V' with (fst (extend a p gen V dst)) by (rewrite E'; easy).
-all: apply IHsrc. assert(Ha := H a); rewrite E in Ha; destruct Ha; subst.
+revert V new; simple_ind try.
+destruct (lookup V a) eqn:E. destruct (extend _) as [V' new'] eqn:E'.
+replace V' with (fst (extend a p gen V new)) by (rewrite E'; easy).
+all: apply IHtry. assert(Ha := H a); rewrite E in Ha; destruct Ha; subst.
 apply sound_extend; easy. easy.
 Qed.
 
-Lemma sound_loop V src n :
-  Sound V -> Sound (loop V src n).
+Lemma sound_loop V try n :
+  Sound V -> Sound (loop V try n).
 Proof.
-revert V src; simple_ind n.
-destruct (extend_loop _) as [V' src'] eqn:E.
-replace V' with (fst (extend_loop V src [])) by (rewrite E; easy).
-destruct src'. apply sound_extend_loop, H.
+revert V try; simple_ind n.
+destruct (extend_loop _) as [V' new] eqn:E.
+replace V' with (fst (extend_loop V try [])) by (rewrite E; easy).
+destruct new. apply sound_extend_loop, H.
 apply IHn, sound_extend_loop, H.
 Qed.
 
@@ -125,40 +125,70 @@ Section Completeness.
 
 Local Open Scope nat.
 
+(* The vector and the new points are an intermediary result. *)
+Definition Intermediary (V : vector) new := Forall (λ i, Defined V i) new /\
+  ∀i, Defined V i -> In i new \/ ∀σ, In σ gen -> Defined V σ⋅i.
+
 (* The vector contains the full orbit. *)
-Definition Complete (V : vector) := ∀π, Generates gen π -> Contains V π⋅k.
+Definition Complete (V : vector) :=
+  ∀π, Generates gen π -> Defined V π⋅k.
 
-Lemma complete_extend_loop_keep V src dst i :
-  Contains V i -> Contains (fst (extend_loop V src dst)) i.
+Lemma defined_extend_loop V try new i :
+  Defined V i -> Defined (fst (extend_loop V try new)) i.
 Proof.
 Admitted.
 
-Lemma complete_loop_keep V src n i :
-  Contains V i -> Contains (loop V src n) i.
+Lemma defined_loop V try m n i :
+  Defined (loop V try m) i -> m <= n -> Defined (loop V try n) i.
 Proof.
 Admitted.
 
-Lemma complete_extend_loop_add V src dst V' dst' σ i:
-  In σ gen -> In i src ->
-  extend_loop V src dst = (V', dst') ->
-  ¬Contains V σ⋅i -> Contains V' σ⋅i /\ In σ⋅i dst'.
+Lemma intermediary_extend_loop V try new V' try' :
+  extend_loop V try new = (V', try') ->
+  Intermediary V try -> Intermediary V' try'.
 Proof.
 Admitted.
 
-Lemma complete_loop V src i w :
-  w ⊆ gen -> In i src -> Contains V i ->
-  Contains (loop V src (length w)) (apply' w i).
+Lemma defined_not_new V try new i :
+  Defined V i -> ¬In i (snd (extend_loop V try new)).
 Proof.
-apply rev_ind with (l:=w); clear w; [intros|intros σ w; intros]; simpl. easy.
-apply incl_app_inv in H0 as []; apply H in H2; try easy; clear H0 H1.
 Admitted.
+
+Lemma finished_intermediary V w i :
+  Intermediary V [] -> Defined V i -> w ⊆ gen -> Defined V (apply' w i).
+Proof.
+Admitted.
+
+Lemma complete_loop V try i w :
+  w ⊆ gen -> Intermediary V try -> Defined V i ->
+  Defined (loop V try (length w)) (apply' w i).
+Proof.
+revert V try i; induction w as [|σ w]; [easy|intros; simpl loop].
+destruct (extend_loop _) as [V' new] eqn:E.
+assert(Intermediary V' new). eapply intermediary_extend_loop; [apply E|easy].
+eapply defined_extend_loop in H1 as H3; rewrite E in H3; simpl in H3.
+eapply defined_not_new in H1 as H4; rewrite E in H4; simpl in H4.
+destruct new as [|j new]. apply finished_intermediary; easy.
+apply incl_cons_inv in H. simpl; apply IHw; try easy.
+destruct H2 as [_ ?]; apply H2 in H3 as []; [easy|].
+apply H3; easy.
+Qed.
 
 Theorem complete_build n :
   size (union_range gen) <= n -> Complete (build n).
 Proof.
 intros H π [w []]; unfold build.
 destruct (short_connecting_word w k) as [w' [? []]].
+assert(w' ⊆ gen) by eauto with datatypes.
 rewrite H1, apply_compose', <-H4.
+eapply defined_loop. apply complete_loop. easy.
+- split. apply Forall_cons. rewrite lookup_insert_eq; easy. auto.
+  intros. rewrite lookup_insert in H6.
+  destruct (k =? i)%positive eqn:E; [|easy].
+  convert_bool; subst; left; apply in_eq.
+- rewrite lookup_insert_eq; easy.
+- etransitivity; [|apply H].
+  admit.
 Admitted.
 
 End Completeness.
