A2_lists.v
@@ -77,5 +77,5 @@ End Well_founded_induction.
 
 End Lists.
 
-Global Hint Resolve incl_nil_l incl_cons incl_app firstn_incl skipn_incl : incl.
+Global Hint Resolve incl_nil_l firstn_incl skipn_incl : datatypes.
 Hint Rewrite firstn_length skipn_length : list.
