B3_word.v
@@ -77,7 +77,7 @@ apply map_singleton_eq in H2, H4; clear H1 H3 H.
 2-5: rewrite map_length, seq_length; easy.
 (* Give the shortened word. *)
 exists (firstn (1 + n0) w ++ skipn (1 + (n0 + 1 + n1)) w); repeat split.
-auto with incl. simpl_list; lia.
+auto with datatypes. simpl_list; lia.
 rewrite fold_left_app, H2, <-H4.
 rewrite <-fold_left_skipn; easy.
 Qed.
